@prefix : <http://www.semanticweb.org/owl/owlapi/turtle#> .
@prefix owl: <http://www.w3.org/2002/07/owl#> .
@prefix rdf: <http://www.w3.org/1999/02/22-rdf-syntax-ns#> .
@prefix xml: <http://www.w3.org/XML/1998/namespace> .
@prefix xsd: <http://www.w3.org/2001/XMLSchema#> .
@prefix rdfs: <http://www.w3.org/2000/01/rdf-schema#> .
@prefix LoSe_ODP: <https://github.com/Michael-Gloeckner/LoSeOn#> .
@base <https://github.com/Michael-Gloeckner/LoSe_ODP> .

<https://github.com/Michael-Gloeckner/LoSe_ODP> rdf:type owl:Ontology ;
                                                
                                                rdfs:label "LoSe_ODP"@en ,
                                                           "Logistics Service"@en ;
                                                
                                                owl:versionInfo "0.2"^^xsd:string ;
                                                
                                                rdfs:comment "This is an ontology design pattern for logistics services."@en ;
                                                
                                                owl:versionInfo "created by Michael Gl√∂ckner"@en .


#################################################################
#
#    Object Properties
#
#################################################################


###  https://github.com/Michael-Gloeckner/LoSe_ODP#IsConnectedBy

<https://github.com/Michael-Gloeckner/LoSe_ODP#IsConnectedBy> rdf:type owl:ObjectProperty ;
                                                              
                                                              rdfs:label "isConnectedBy"@en ;
                                                              
                                                              rdfs:comment "describes the connection of something by something"@en ;
                                                              
                                                              rdfs:range <https://github.com/Michael-Gloeckner/LoSe_ODP#Flow> ;
                                                              
                                                              rdfs:domain <https://github.com/Michael-Gloeckner/LoSe_ODP#LogisticsService> .



###  https://github.com/Michael-Gloeckner/LoSe_ODP#IsConsumedBy

<https://github.com/Michael-Gloeckner/LoSe_ODP#IsConsumedBy> rdf:type owl:ObjectProperty ;
                                                             
                                                             rdfs:label "isConsumedBy"@en ;
                                                             
                                                             rdfs:comment "describes the consumption of something by something"@en ;
                                                             
                                                             rdfs:domain <https://github.com/Michael-Gloeckner/LoSe_ODP#LogisticsService> ;
                                                             
                                                             rdfs:range <https://github.com/Michael-Gloeckner/LoSe_ODP#LogisticsService> ,
                                                                        <https://github.com/Michael-Gloeckner/LoSe_ODP#LogisticsStakeholder> ;
                                                             
                                                             rdfs:domain <https://github.com/Michael-Gloeckner/LoSe_ODP#Resource> .



###  https://github.com/Michael-Gloeckner/LoSe_ODP#IsContrainedBy

<https://github.com/Michael-Gloeckner/LoSe_ODP#IsContrainedBy> rdf:type owl:ObjectProperty ;
                                                               
                                                               rdfs:label "isContrainedBy"@en ;
                                                               
                                                               rdfs:comment "describes constrain of something by something"@en ;
                                                               
                                                               rdfs:range <https://github.com/Michael-Gloeckner/LoSe_ODP#Contraints> ;
                                                               
                                                               rdfs:domain <https://github.com/Michael-Gloeckner/LoSe_ODP#LogisticsService> .



###  https://github.com/Michael-Gloeckner/LoSe_ODP#IsEnabledBy

<https://github.com/Michael-Gloeckner/LoSe_ODP#IsEnabledBy> rdf:type owl:ObjectProperty ;
                                                            
                                                            rdfs:label "isEnabledBy"@en ;
                                                            
                                                            rdfs:comment "describes the enabling of sommething by sommething"@en ;
                                                            
                                                            rdfs:domain <https://github.com/Michael-Gloeckner/LoSe_ODP#Flow> ;
                                                            
                                                            rdfs:range <https://github.com/Michael-Gloeckner/LoSe_ODP#Resource> ;
                                                            
                                                            rdfs:domain <https://github.com/Michael-Gloeckner/LoSe_ODP#Transformation> .



###  https://github.com/Michael-Gloeckner/LoSe_ODP#IsMeasuredBy

<https://github.com/Michael-Gloeckner/LoSe_ODP#IsMeasuredBy> rdf:type owl:ObjectProperty ;
                                                             
                                                             rdfs:label "isMeasuredBy"@en ;
                                                             
                                                             rdfs:comment "describes measurement of something by something"@en ;
                                                             
                                                             rdfs:domain <https://github.com/Michael-Gloeckner/LoSe_ODP#LogisticsService> ;
                                                             
                                                             rdfs:range <https://github.com/Michael-Gloeckner/LoSe_ODP#SLA> .



###  https://github.com/Michael-Gloeckner/LoSe_ODP#IsPerformedBy

<https://github.com/Michael-Gloeckner/LoSe_ODP#IsPerformedBy> rdf:type owl:ObjectProperty ;
                                                              
                                                              rdfs:label "isPerformedBy"@en ;
                                                              
                                                              rdfs:comment "describes the performance of something by something"@en ;
                                                              
                                                              rdfs:range <https://github.com/Michael-Gloeckner/LoSe_ODP#Active> ,
                                                                         <https://github.com/Michael-Gloeckner/LoSe_ODP#LogisticsService> ;
                                                              
                                                              rdfs:domain <https://github.com/Michael-Gloeckner/LoSe_ODP#Transformation> .



###  https://github.com/Michael-Gloeckner/LoSe_ODP#IsProvidedBy

<https://github.com/Michael-Gloeckner/LoSe_ODP#IsProvidedBy> rdf:type owl:ObjectProperty ;
                                                             
                                                             rdfs:label "isProvidedBy"@en ;
                                                             
                                                             rdfs:comment "describes the provision of something by something"@en ;
                                                             
                                                             rdfs:domain <https://github.com/Michael-Gloeckner/LoSe_ODP#LogisticsService> ;
                                                             
                                                             rdfs:range <https://github.com/Michael-Gloeckner/LoSe_ODP#LogisticsStakeholder> .





#################################################################
#
#    Classes
#
#################################################################


###  https://github.com/Michael-Gloeckner/LoSe_ODP#Active

<https://github.com/Michael-Gloeckner/LoSe_ODP#Active> rdf:type owl:Class ;
                                                       
                                                       rdfs:label "Active"@en ;
                                                       
                                                       rdfs:subClassOf <https://github.com/Michael-Gloeckner/LoSe_ODP#Power> ;
                                                       
                                                       rdfs:comment "An Active Resource posseses the ability of transforming a logistics entity by itself."@en .



###  https://github.com/Michael-Gloeckner/LoSe_ODP#Character

<https://github.com/Michael-Gloeckner/LoSe_ODP#Character> rdf:type owl:Class ;
                                                          
                                                          rdfs:label "Character"@en ;
                                                          
                                                          rdfs:subClassOf <https://github.com/Michael-Gloeckner/LoSe_ODP#Resource> ;
                                                          
                                                          rdfs:comment "The Character describes the consistence of a Resource. It is either Informational OR Physical."@en .



###  https://github.com/Michael-Gloeckner/LoSe_ODP#Contraints

<https://github.com/Michael-Gloeckner/LoSe_ODP#Contraints> rdf:type owl:Class ;
                                                           
                                                           rdfs:label "Constraints"@en ;
                                                           
                                                           rdfs:comment "Contraints define external requirements that have to be fulfilled by a logistics service. They are either of mandatory (such as official laws) or non-mandatory nature (such as customer requirements)."@en .



###  https://github.com/Michael-Gloeckner/LoSe_ODP#Control

<https://github.com/Michael-Gloeckner/LoSe_ODP#Control> rdf:type owl:Class ;
                                                        
                                                        rdfs:label "Control"@en ;
                                                        
                                                        rdfs:subClassOf <https://github.com/Michael-Gloeckner/LoSe_ODP#Flow> ;
                                                        
                                                        rdfs:comment "Control is the Flow of information in order to trigger following LogisticsService."@en .



###  https://github.com/Michael-Gloeckner/LoSe_ODP#Cost

<https://github.com/Michael-Gloeckner/LoSe_ODP#Cost> rdf:type owl:Class ;
                                                     
                                                     rdfs:label "Cost"@en ;
                                                     
                                                     rdfs:subClassOf <https://github.com/Michael-Gloeckner/LoSe_ODP#Transformation> ;
                                                     
                                                     rdfs:comment "A LogisticsService tranforms costs of the overall service in a certain kind of way. Usually Costs increase by the usage of a Service."@en .



###  https://github.com/Michael-Gloeckner/LoSe_ODP#Economic

<https://github.com/Michael-Gloeckner/LoSe_ODP#Economic> rdf:type owl:Class ;
                                                         
                                                         rdfs:label "Economic"@en ;
                                                         
                                                         rdfs:subClassOf <https://github.com/Michael-Gloeckner/LoSe_ODP#NonMandatory> ;
                                                         
                                                         rdfs:comment "Economic contraints aim at delivering complex logistics services in a cheap way."@en .



###  https://github.com/Michael-Gloeckner/LoSe_ODP#Environmental

<https://github.com/Michael-Gloeckner/LoSe_ODP#Environmental> rdf:type owl:Class ;
                                                              
                                                              rdfs:label "Environmental"@en ;
                                                              
                                                              rdfs:subClassOf <https://github.com/Michael-Gloeckner/LoSe_ODP#NonMandatory> ;
                                                              
                                                              rdfs:comment "Environmental constraints aim at delivering complex logistics services in a einvironmentally friendly way, e.g. with a reduced carbon footprint."@en .



###  https://github.com/Michael-Gloeckner/LoSe_ODP#Flow

<https://github.com/Michael-Gloeckner/LoSe_ODP#Flow> rdf:type owl:Class ;
                                                     
                                                     rdfs:label "Flow"@en ;
                                                     
                                                     rdfs:comment "The several flows connect two or more logistics services with each other. Different kinds of flows can be distinguished."@en .



###  https://github.com/Michael-Gloeckner/LoSe_ODP#Information

<https://github.com/Michael-Gloeckner/LoSe_ODP#Information> rdf:type owl:Class ;
                                                            
                                                            rdfs:label "Information"@en ;
                                                            
                                                            rdfs:subClassOf <https://github.com/Michael-Gloeckner/LoSe_ODP#Transformation> ;
                                                            
                                                            rdfs:comment "A LogisticsService could transform Information in a certain kind of way."@en .



###  https://github.com/Michael-Gloeckner/LoSe_ODP#Informational

<https://github.com/Michael-Gloeckner/LoSe_ODP#Informational> rdf:type owl:Class ;
                                                              
                                                              rdfs:label "Informational"@en ;
                                                              
                                                              rdfs:subClassOf <https://github.com/Michael-Gloeckner/LoSe_ODP#Character> ,
                                                                              <https://github.com/Michael-Gloeckner/LoSe_ODP#Flow> ;
                                                              
                                                              rdfs:comment "Either one of the Flows connecting LogisticsService or the characteristics of a certain Resource could be Informational."@en .



###  https://github.com/Michael-Gloeckner/LoSe_ODP#Location

<https://github.com/Michael-Gloeckner/LoSe_ODP#Location> rdf:type owl:Class ;
                                                         
                                                         rdfs:label "Location"@en ;
                                                         
                                                         rdfs:subClassOf <https://github.com/Michael-Gloeckner/LoSe_ODP#Transformation> ;
                                                         
                                                         rdfs:comment "A LogisticsService could transform Location in a certain kind of way."@en .



###  https://github.com/Michael-Gloeckner/LoSe_ODP#LogisticsService

<https://github.com/Michael-Gloeckner/LoSe_ODP#LogisticsService> rdf:type owl:Class ;
                                                                 
                                                                 rdfs:label "LogisticsService"@en ;
                                                                 
                                                                 rdfs:comment """A Logistics Service is characterized by general service characteristics. This includes a pre-defined set of inputs, outputs and transformations that take place during its execution. Further important is the usage of resources and the application of knowledge and skills within activities or processes in order to generate benefit for another entity or for the entity itself.

A Logistics Service is a Service conducted within the logistics domain and logistics purpose."""@en .



###  https://github.com/Michael-Gloeckner/LoSe_ODP#LogisticsStakeholder

<https://github.com/Michael-Gloeckner/LoSe_ODP#LogisticsStakeholder> rdf:type owl:Class ;
                                                                     
                                                                     rdfs:label "LogisticsStakeholder"@en ;
                                                                     
                                                                     rdfs:comment "A LogisticsStakeholder is a natural or a legal person involved in the planning, operation or monitoring of a LogisticsService. It either provides, uses or manages the service or is in another way connected to it."@en .



###  https://github.com/Michael-Gloeckner/LoSe_ODP#Mandatory

<https://github.com/Michael-Gloeckner/LoSe_ODP#Mandatory> rdf:type owl:Class ;
                                                          
                                                          rdfs:label "Mandatory"@en ;
                                                          
                                                          rdfs:subClassOf <https://github.com/Michael-Gloeckner/LoSe_ODP#Contraints> ;
                                                          
                                                          owl:disjointWith <https://github.com/Michael-Gloeckner/LoSe_ODP#NonMandatory> ;
                                                          
                                                          rdfs:comment "Mandatory contraints are requirements by official, public or governmental institutions."@en .



###  https://github.com/Michael-Gloeckner/LoSe_ODP#NonMandatory

<https://github.com/Michael-Gloeckner/LoSe_ODP#NonMandatory> rdf:type owl:Class ;
                                                             
                                                             rdfs:label "NonMandatory"@en ;
                                                             
                                                             rdfs:subClassOf <https://github.com/Michael-Gloeckner/LoSe_ODP#Contraints> ;
                                                             
                                                             rdfs:comment "Non-mandatory contraints are requirements by customers. They are not obligatory like the mandatory contraints from legal institutions."@en .



###  https://github.com/Michael-Gloeckner/LoSe_ODP#Passive

<https://github.com/Michael-Gloeckner/LoSe_ODP#Passive> rdf:type owl:Class ;
                                                        
                                                        rdfs:label "Passive"@en ;
                                                        
                                                        rdfs:subClassOf <https://github.com/Michael-Gloeckner/LoSe_ODP#Power> ;
                                                        
                                                        rdfs:comment "An Passive Resource does not posses the ability of transforming a logistics entity by itself. It is transformed by an Active Resource."@en .



###  https://github.com/Michael-Gloeckner/LoSe_ODP#Physical

<https://github.com/Michael-Gloeckner/LoSe_ODP#Physical> rdf:type owl:Class ;
                                                         
                                                         rdfs:label "Physical"@en ;
                                                         
                                                         rdfs:subClassOf <https://github.com/Michael-Gloeckner/LoSe_ODP#Character> ,
                                                                         <https://github.com/Michael-Gloeckner/LoSe_ODP#Flow> ;
                                                         
                                                         rdfs:comment "Either one of the Flows connecting LogisticsService or the characteristics of a certain Resource could be Physical."@en .



###  https://github.com/Michael-Gloeckner/LoSe_ODP#Power

<https://github.com/Michael-Gloeckner/LoSe_ODP#Power> rdf:type owl:Class ;
                                                      
                                                      rdfs:label "Power"@en ;
                                                      
                                                      rdfs:subClassOf <https://github.com/Michael-Gloeckner/LoSe_ODP#Resource> ;
                                                      
                                                      rdfs:comment "The Power describes the ability of a Resource. It is either Active OR Passive."@en .



###  https://github.com/Michael-Gloeckner/LoSe_ODP#Product

<https://github.com/Michael-Gloeckner/LoSe_ODP#Product> rdf:type owl:Class ;
                                                        
                                                        rdfs:label "Product"@en ;
                                                        
                                                        rdfs:subClassOf <https://github.com/Michael-Gloeckner/LoSe_ODP#Transformation> ;
                                                        
                                                        rdfs:comment "A LogisticsService could transform Product in a certain kind of way."@en .



###  https://github.com/Michael-Gloeckner/LoSe_ODP#Quality

<https://github.com/Michael-Gloeckner/LoSe_ODP#Quality> rdf:type owl:Class ;
                                                        
                                                        rdfs:label "Quality"@en ;
                                                        
                                                        rdfs:subClassOf <https://github.com/Michael-Gloeckner/LoSe_ODP#Transformation> ;
                                                        
                                                        rdfs:comment "A LogisticsService could transform Quality of a Product in a certain kind of way."@en .



###  https://github.com/Michael-Gloeckner/LoSe_ODP#Quantity

<https://github.com/Michael-Gloeckner/LoSe_ODP#Quantity> rdf:type owl:Class ;
                                                         
                                                         rdfs:label "Quantity"@en ;
                                                         
                                                         rdfs:subClassOf <https://github.com/Michael-Gloeckner/LoSe_ODP#Transformation> ;
                                                         
                                                         rdfs:comment "A LogisticsService could transform Quantity of a Product in a certain kind of way."@en .



###  https://github.com/Michael-Gloeckner/LoSe_ODP#Resource

<https://github.com/Michael-Gloeckner/LoSe_ODP#Resource> rdf:type owl:Class ;
                                                         
                                                         rdfs:label "Resource"@en ;
                                                         
                                                         rdfs:comment "A Resource is consumed during the conduction of a LogisticsService. It is either available again afterward (such as warehouse capacity or a truck) or not (such as some kind of one-way packaging)."@en .



###  https://github.com/Michael-Gloeckner/LoSe_ODP#SLA

<https://github.com/Michael-Gloeckner/LoSe_ODP#SLA> rdf:type owl:Class ;
                                                    
                                                    rdfs:label "ServiceLevelAgreements"@en ;
                                                    
                                                    rdfs:comment "ServiceLevelAgreements determine the quality of the service, e.g. lead time, accuracy."@en .



###  https://github.com/Michael-Gloeckner/LoSe_ODP#Social

<https://github.com/Michael-Gloeckner/LoSe_ODP#Social> rdf:type owl:Class ;
                                                       
                                                       rdfs:label "Social"@en ;
                                                       
                                                       rdfs:subClassOf <https://github.com/Michael-Gloeckner/LoSe_ODP#NonMandatory> ;
                                                       
                                                       rdfs:comment "Social contraints aim at delivering complex logistics services in a socially reasonable way, e.g. with a guaranteed minimum wage."@en .



###  https://github.com/Michael-Gloeckner/LoSe_ODP#Time

<https://github.com/Michael-Gloeckner/LoSe_ODP#Time> rdf:type owl:Class ;
                                                     
                                                     rdfs:label "Time"@en ;
                                                     
                                                     rdfs:subClassOf <https://github.com/Michael-Gloeckner/LoSe_ODP#Transformation> ;
                                                     
                                                     rdfs:comment "Time describes the temporal starting and ending points of a LogisticsService."@en ;
                                                     
                                                     rdfs:seeAlso "http://www.ontologydesignpatterns.org/cp/owl/timeinterval.owl"@en .



###  https://github.com/Michael-Gloeckner/LoSe_ODP#Transformation

<https://github.com/Michael-Gloeckner/LoSe_ODP#Transformation> rdf:type owl:Class ;
                                                               
                                                               rdfs:label "Transformation"@en ;
                                                               
                                                               rdfs:comment "Transformation contains the possible dimensions that could be changed during a LogisticsService."@en .



[ rdfs:label "LoSeOn"^^xsd:string
] .

###  Generated by the OWL API (version 3.4.2) http://owlapi.sourceforge.net

